CHANGE: clock updates for client events, and reading lst

txn-data-consistency/EP+_TCCv.thy
@@ -11,6 +11,7 @@ subsection \<open>State\<close>
 type_synonym key = key
 type_synonym tstmp = nat
 type_synonym dep_set = "txid set"
+type_synonym readerset = "(txid0 \<times> tstmp \<times> tstmp) set" \<comment> \<open>t, svr_clock at read, svr lst at read\<close>
 
 \<comment> \<open>Client State\<close>
 datatype 'v txn_state =
@@ -29,10 +30,10 @@ definition dep_set_init :: dep_set where
 
 \<comment> \<open>Server State\<close>
 datatype 'v ver_state = No_Ver | Prep (get_ts: tstmp) (get_val: 'v)
-  | Commit (get_ts: tstmp) (get_val: 'v) "txid0 set"
+  | Commit (get_ts: tstmp) (get_sclk: tstmp) (get_lst: tstmp) (get_val: 'v) readerset
 
 fun is_committed :: "'v ver_state \<Rightarrow> bool" where
-  "is_committed (Commit _ _ _) = True" |
+  "is_committed (Commit _ _ _ _ _) = True" |
   "is_committed _ = False"
 
 fun is_prepared :: "'v ver_state \<Rightarrow> bool" where
@@ -44,7 +45,7 @@ type_synonym 'v wtxn_state = "txid \<Rightarrow> 'v ver_state"
 record 'v svr_conf =
   svr_state :: "'v wtxn_state"
   svr_clock :: tstmp
-  lst :: tstmp
+  svr_lst :: tstmp
 
 abbreviation wtxns_emp :: "txid \<Rightarrow> 'v ver_state" where
   "wtxns_emp \<equiv> (\<lambda>t. No_Ver)"
@@ -74,10 +75,10 @@ fun get_sn_w :: "txid \<Rightarrow> sqn" where
   "get_sn_w T0 = undefined" |
   "get_sn_w (Tn (Tn_cl sn cl)) = sn"
 
-fun get_rs :: "'v ver_state \<Rightarrow> txid0 set" where
+fun get_rs :: "'v ver_state \<Rightarrow> readerset" where
   "get_rs No_Ver = undefined" |
   "get_rs (Prep _ _) = {}" |
-  "get_rs (Commit _ _ rs) = rs"
+  "get_rs (Commit _ _ _ _ rs) = rs"
 
 
 subsubsection \<open>Customised dom and ran functions for svr_state\<close>
@@ -88,7 +89,7 @@ definition wtxns_dom :: "'v wtxn_state \<Rightarrow> txid set" where
 definition wtxns_vran :: "'v wtxn_state \<Rightarrow> 'v set" where
   "wtxns_vran wtxns \<equiv> {get_val (wtxns t) | t. t \<in> wtxns_dom wtxns}"
 
-definition wtxns_rsran :: "'v wtxn_state \<Rightarrow> txid0 set" where
+definition wtxns_rsran :: "'v wtxn_state \<Rightarrow> readerset" where
   "wtxns_rsran wtxns \<equiv> \<Union>{get_rs (wtxns t) | t. t \<in> wtxns_dom wtxns}"
 
 
@@ -129,9 +130,9 @@ definition read_at :: "'v wtxn_state \<Rightarrow> tstmp \<Rightarrow> cl_id \<R
 
 subsubsection \<open>Helper functions\<close>
 
-definition add_to_readerset :: "'v wtxn_state \<Rightarrow> txid0 \<Rightarrow> txid \<Rightarrow> 'v wtxn_state" where
-  "add_to_readerset wtxns t t_wr \<equiv> (case wtxns t_wr of
-    Commit cts v rs \<Rightarrow> wtxns (t_wr := Commit cts v (insert t rs)) |
+definition add_to_readerset :: "'v wtxn_state \<Rightarrow> txid0 \<Rightarrow> tstmp \<Rightarrow> tstmp \<Rightarrow> txid \<Rightarrow> 'v wtxn_state" where
+  "add_to_readerset wtxns t rts rlst t_wr \<equiv> (case wtxns t_wr of
+    Commit cts ts lst v rs \<Rightarrow> wtxns (t_wr := Commit cts ts lst v (insert (t, rts, rlst) rs)) |
     _ \<Rightarrow> wtxns)"
 
 definition pending_wtxns_ts :: "'v wtxn_state \<Rightarrow> tstmp set" where
@@ -159,7 +160,7 @@ definition ext_corder :: "txid \<Rightarrow> (key \<rightharpoonup> 'v) \<Righta
 subsection \<open>Events\<close>
 
 datatype 'v ev =
-  RInvoke cl_id "key set" | Read cl_id key 'v txid | RDone cl_id "key \<rightharpoonup> 'v" sqn view |
+  RInvoke cl_id "key set" | Read cl_id key 'v txid tstmp tstmp | RDone cl_id "key \<rightharpoonup> 'v" sqn view |
   WInvoke cl_id "key \<rightharpoonup> 'v" | WCommit cl_id "key \<rightharpoonup> 'v" tstmp sqn view | WDone cl_id "key \<rightharpoonup> 'v" |
   RegR key txid0 txid tstmp | PrepW key txid 'v | CommitW key txid 'v tstmp | Skip2
 
@@ -194,26 +195,26 @@ definition read_invoke :: "cl_id \<Rightarrow> key set \<Rightarrow> ('v, 'm) gl
     s' = read_invoke_U cl keys s"
 
 abbreviation read_G where
-  "read_G cl k v t s \<equiv> 
+  "read_G cl k v t rts rlst s \<equiv> 
     \<comment> \<open>reads server k's value v for client transaction, lst, and svr_clock\<close>
-    (\<exists>cts rs. svr_state (svrs s k) t = Commit cts v rs \<and> get_txn s cl \<in> rs) \<and>
+    (\<exists>cts ts lst rs. svr_state (svrs s k) t = Commit cts ts lst v rs \<and> (get_txn s cl, rts, rlst) \<in> rs) \<and>
     (\<exists>keys kv_map. cl_state (cls s cl) = RtxnInProg keys kv_map \<and> k \<in> keys \<and> kv_map k = None)"
 
 abbreviation read_U where
-  "read_U cl k v s \<equiv>
+  "read_U cl k v rts rlst s \<equiv>
     s \<lparr> cls := (cls s)
       (cl := cls s cl \<lparr>
         cl_state :=
           (case cl_state (cls s cl) of RtxnInProg keys kv_map \<Rightarrow> RtxnInProg keys (kv_map (k \<mapsto> v))),
-        cl_clock := Suc (max (cl_clock (cls s cl)) (svr_clock (svrs s k))),
-        lst_map := (lst_map (cls s cl)) (k := lst (svrs s k))
+        cl_clock := Suc (max (cl_clock (cls s cl)) rts),
+        lst_map := (lst_map (cls s cl)) (k := rlst)
       \<rparr>)
     \<rparr>"
 
-definition read :: "cl_id \<Rightarrow> key \<Rightarrow> 'v \<Rightarrow> txid \<Rightarrow> ('v, 'm) global_conf_scheme \<Rightarrow> ('v, 'm) global_conf_scheme \<Rightarrow> bool" where
-  "read cl k v t s s' \<equiv>
-    read_G cl k v t s \<and>
-    s' = read_U cl k v s"
+definition read :: "cl_id \<Rightarrow> key \<Rightarrow> 'v \<Rightarrow> txid \<Rightarrow> tstmp \<Rightarrow> tstmp \<Rightarrow> ('v, 'm) global_conf_scheme \<Rightarrow> ('v, 'm) global_conf_scheme \<Rightarrow> bool" where
+  "read cl k v t rts rlst s s' \<equiv>
+    read_G cl k v t rts rlst s \<and>
+    s' = read_U cl k v rts rlst s"
 
 abbreviation read_done_G where
   "read_done_G cl kv_map sn s \<equiv>
@@ -268,7 +269,7 @@ definition write_commit_U where
     s \<lparr> cls := (cls s)
       (cl := cls s cl \<lparr>
         cl_state := WtxnCommit cts kv_map,
-        cl_clock := Suc (max (cl_clock (cls s cl)) cts), \<comment> \<open>Why not max of all involved server svr_clocks\<close>
+        cl_clock := Suc (max (cl_clock (cls s cl)) cts),
         cl_ctx := insert (get_wtxn s cl) (cl_ctx (cls s cl))
       \<rparr>), 
       wtxn_deps := (wtxn_deps s) (get_wtxn s cl := cl_ctx (cls s cl))
@@ -282,7 +283,7 @@ definition write_commit :: "cl_id \<Rightarrow> (key \<rightharpoonup> 'v) \<Rig
 definition write_done_G where
   "write_done_G cl kv_map s \<equiv>
     (\<exists>cts. cl_state (cls s cl) = WtxnCommit cts kv_map \<and>
-      (\<forall>k\<in>dom kv_map. \<exists>v rs. svr_state (svrs s k) (get_wtxn s cl) = Commit cts v rs \<and>
+      (\<forall>k\<in>dom kv_map. \<exists>ts lst v rs. svr_state (svrs s k) (get_wtxn s cl) = Commit cts ts lst v rs \<and>
          kv_map k = Some v))"
 
 definition write_done_U where
@@ -291,8 +292,8 @@ definition write_done_U where
       (cl := cls s cl \<lparr>
         cl_state := Idle,
         cl_sn := Suc (cl_sn (cls s cl)),
-        cl_clock := Suc (max (cl_clock (cls s cl)) (Max {svr_clock (svrs s k) | k. k \<in> dom kv_map})),
-        lst_map := (\<lambda>k. if kv_map k = None then lst_map (cls s cl) k else lst (svrs s k))
+        cl_clock := Suc (max (cl_clock (cls s cl)) (Max {get_sclk (svr_state (svrs s k) (get_wtxn s cl)) | k. k \<in> dom kv_map})),
+        lst_map := (\<lambda>k. if kv_map k = None then lst_map (cls s cl) k else get_lst (svr_state (svrs s k) (get_wtxn s cl)))
       \<rparr>)
     \<rparr>"
 
@@ -315,7 +316,7 @@ abbreviation register_read_U where
   "register_read_U svr t t_wr s\<equiv>
     s \<lparr> svrs := (svrs s)
       (svr := svrs s svr \<lparr>
-        svr_state := add_to_readerset (svr_state (svrs s svr)) t t_wr,
+        svr_state := add_to_readerset (svr_state (svrs s svr)) t (svr_clock (svrs s svr)) (svr_lst (svrs s svr)) t_wr,
         svr_clock := Suc (max (svr_clock (svrs s svr)) (cl_clock (cls s (get_cl t))))
       \<rparr>)
     \<rparr>"
@@ -356,11 +357,12 @@ definition commit_write_U where
   "commit_write_U svr t v cts s \<equiv>
     s \<lparr> svrs := (svrs s)
       (svr := svrs s svr \<lparr>
-        svr_state := (svr_state (svrs s svr))(t := Commit cts v {}),
+        svr_state := (svr_state (svrs s svr))(t := Commit cts (svr_clock (svrs s svr)) (svr_lst (svrs s svr)) v {}),
         svr_clock := Suc (max (svr_clock (svrs s svr)) (cl_clock (cls s (get_cl_w t)))),
-        lst := if pending_wtxns_ts ((svr_state (svrs s svr)) (t := Commit cts v {})) = {}
+        svr_lst := if pending_wtxns_ts ((svr_state (svrs s svr)) (t := Commit cts (svr_clock (svrs s svr)) (svr_lst (svrs s svr)) v {})) = {}
                then svr_clock (svrs s svr)
-               else Min (pending_wtxns_ts ((svr_state (svrs s svr)) (t := Commit cts v {})))
+               else Min (pending_wtxns_ts ((svr_state (svrs s svr))
+                      (t := Commit cts (svr_clock (svrs s svr)) (svr_lst (svrs s svr)) v {})))
       \<rparr>)
     \<rparr>"
 
@@ -380,7 +382,7 @@ definition state_init :: "'v global_conf" where
                   cl_ctx = dep_set_init,
                   gst = 0,
                   lst_map = (\<lambda>svr. 0) \<rparr>),
-    svrs = (\<lambda>svr. \<lparr> svr_state = (\<lambda>t. No_Ver) (T0 := Commit 0 undefined {}),
+    svrs = (\<lambda>svr. \<lparr> svr_state = (\<lambda>t. No_Ver) (T0 := Commit 0 0 0 undefined {}),
                     svr_clock = 0,
                     lst = 0 \<rparr>),
     wtxn_deps = (\<lambda>t. {})
@@ -388,7 +390,7 @@ definition state_init :: "'v global_conf" where
 
 fun state_trans :: "('v, 'm) global_conf_scheme \<Rightarrow> 'v ev \<Rightarrow> ('v, 'm) global_conf_scheme \<Rightarrow> bool" where
   "state_trans s (RInvoke cl keys)          s' \<longleftrightarrow> read_invoke cl keys s s'" |
-  "state_trans s (Read cl k v t)            s' \<longleftrightarrow> read cl k v t s s'" |
+  "state_trans s (Read cl k v t rts rlst)        s' \<longleftrightarrow> read cl k v t rts rlst s s'" |
   "state_trans s (RDone cl kv_map sn u'')   s' \<longleftrightarrow> read_done cl kv_map sn s s'" |
   "state_trans s (WInvoke cl kv_map)        s' \<longleftrightarrow> write_invoke cl kv_map s s'" |
   "state_trans s (WCommit cl kv_map cts sn u'') s' \<longleftrightarrow> write_commit cl kv_map cts sn s s'" |
